use context instead of opening new locales + resolve definition name clash + fix proofs by restricting types + fix some proofs manually + us 'm not 'k for mapval | everything verifies now (although maybe a bit slow)

BoogieLang/Ast.thy
@@ -89,12 +89,7 @@ fun is_final :: "('a, 'm) ast_config \<Rightarrow> bool"
 
 text \<open>Small-step semantics\<close>
 
-locale ast =
-  fixes map_select :: "('a::absval, 'm::mapval) val \<Rightarrow> ('a, 'm) val \<Rightarrow> ('a, 'm) val"
-  fixes map_store  :: "('a, 'm) val \<Rightarrow> ('a, 'm) val \<Rightarrow> ('a, 'm) val \<Rightarrow> ('a, 'm) val"
-begin
-
-interpretation semantics map_select map_store .
+context semantics begin
 
 inductive red_bigblock :: "'p proc_context \<Rightarrow> var_context \<Rightarrow> ('a, 'm) fun_interp \<Rightarrow> rtype_env  \<Rightarrow> ast \<Rightarrow> ('a, 'm) ast_config \<Rightarrow> ('a, 'm) ast_config \<Rightarrow> bool" 
   ("_,_,_,_,_ \<turnstile> (\<langle>_\<rangle> \<longrightarrow>/ _)" [51,0,0,0] 81)
@@ -203,16 +198,16 @@ fun init_ast :: "ast \<Rightarrow> ('a, 'm) nstate \<Rightarrow> ('a, 'm) ast_co
     "init_ast [] ns1 = ((BigBlock None [] None None), KStop, Normal ns1)"
   | "init_ast (b#bbs) ns1 = (b, convert_list_to_cont ( bbs) KStop, Normal ns1)"
 
-definition valid_configuration 
-  where "valid_configuration \<Lambda> \<Gamma> \<Omega> posts bb cont state \<equiv> 
+definition ast_valid_configuration
+  where "ast_valid_configuration \<Lambda> \<Gamma> \<Omega> posts bb cont state \<equiv>
          state \<noteq> Failure \<and> 
          (is_final (bb, cont, state) \<longrightarrow> (\<forall>ns'. state = Normal ns' \<longrightarrow> expr_all_sat \<Lambda> \<Gamma> \<Omega> ns' posts))"
 
-definition proc_body_satisfies_spec :: "'p proc_context \<Rightarrow> var_context \<Rightarrow> ('a, 'm) fun_interp \<Rightarrow> rtype_env \<Rightarrow> expr list \<Rightarrow> expr list \<Rightarrow> ast \<Rightarrow> ('a, 'm) nstate \<Rightarrow> bool"
-  where "proc_body_satisfies_spec M \<Lambda> \<Gamma> \<Omega> pres posts ast ns \<equiv>
+definition ast_proc_body_satisfies_spec :: "'p proc_context \<Rightarrow> var_context \<Rightarrow> ('a, 'm) fun_interp \<Rightarrow> rtype_env \<Rightarrow> expr list \<Rightarrow> expr list \<Rightarrow> ast \<Rightarrow> ('a, 'm) nstate \<Rightarrow> bool"
+  where "ast_proc_body_satisfies_spec M \<Lambda> \<Gamma> \<Omega> pres posts ast ns \<equiv>
          expr_all_sat \<Lambda> \<Gamma> \<Omega> ns pres \<longrightarrow> 
           (\<forall> bb cont state. (rtranclp (red_bigblock M \<Lambda> \<Gamma> \<Omega> ast) (init_ast ast ns) (bb, cont, state)) \<longrightarrow> 
-                    valid_configuration \<Lambda> \<Gamma> \<Omega> posts bb cont state)"
+                    ast_valid_configuration \<Lambda> \<Gamma> \<Omega> posts bb cont state)"
 
 fun proc_all_pres :: "ast procedure \<Rightarrow> expr list"
   where "proc_all_pres p = map fst (proc_pres p)"
